finish proof for EqGraph.seq

Core/Ppcc/Basic.lean
@@ -44,6 +44,7 @@ as during the path compression in union-find DS, the explanations are essentiall
 structure Node (G : GlobalEnv) (Δ : KindEnv) where
   payload : (T : Ty) × (K : Kind) ×' (G&Δ ⊢ T : K)
 
+@[simp, grind =]
 def Node.get_ty (n : Node G Δ) : Ty := n.payload.1
 
 structure EqGraphNode (G : GlobalEnv) (Δ : KindEnv) where
@@ -51,49 +52,98 @@ structure EqGraphNode (G : GlobalEnv) (Δ : KindEnv) where
   rank : Nat
   payload : Node G Δ
 
+@[simp, grind =]
 def EqGraphNode.get_ty (n : EqGraphNode G Δ) : Ty := n.payload.get_ty
 
 structure Edge (G : GlobalEnv) (Δ : KindEnv) (Γ : TyEnv) where
   payload : (t : Term) × (T : Ty) ×' G&Δ, Γ ⊢ t : T
 
+@[simp, grind =]
 def Edge.get_term (e : Edge G Δ Γ) : Term := e.payload.1
+
+/-- Parent of a union-find node, defaults to self when the node is a root -/
+def parentD (nodes : List (EqGraphNode G Δ)) (i : Nat) : Nat :=
+  if h : i < nodes.length then nodes[i].parent else i
+
+/-- Rank of a union-find node, defaults to 0 when the node is a root -/
+def rankD (nodes : List (EqGraphNode G Δ)) (i : Nat) : Nat :=
+  if h : i < nodes.length then nodes[i].rank else 0
 
 structure EqGraph (G : GlobalEnv) (Δ : KindEnv) (Γ : TyEnv) where
   nodes : List (EqGraphNode G Δ)
   edges : List (Nat × Nat × Edge G Δ Γ)
+  /-- Validity for parent nodes -/
+  parentD_lt : ∀ {i}, (h : i < nodes.length) → nodes[i].parent < nodes.length
+  /-- Validity for rank -/
+  rankD_lt : ∀ {i}, parentD nodes i ≠ i → rankD node i < rankD nodes (parentD nodes i)
+
 
 instance instMembershipTyEqGraph {G : GlobalEnv} {Δ : KindEnv} {Γ : TyEnv} : Membership Ty (EqGraph G Δ Γ) where
-  mem eG T := T ∈ eG.nodes.map (λ n => n.get_ty)
+  mem eG T := List.elem T (eG.nodes.map (λ n => n.get_ty))
 
-def EqGraph.push {G : GlobalEnv} {Δ : KindEnv} {Γ : TyEnv}(eG : EqGraph G Δ Γ) : Node G Δ -> EqGraph G Δ Γ := sorry
+def EqGraph.elem_node {G : GlobalEnv} {Δ : KindEnv} {Γ : TyEnv} (n : Node G Δ)(eG : EqGraph G Δ Γ) : Bool :=
+  List.elem (n.get_ty) (eG.nodes.map (λ n => n.get_ty))
+
+def EqGraph.push {G : GlobalEnv} {Δ : KindEnv} {Γ : TyEnv}(eG : EqGraph G Δ Γ) (n : Node G Δ) : EqGraph G Δ Γ :=
+  if eG.elem_node n
+  then eG
+  else { nodes := eG.nodes ++ [⟨eG.nodes.length, 0, n⟩]
+       , edges := eG.edges
+       , parentD_lt := by intro h1 h2; sorry
+       , rankD_lt := sorry}
 
 theorem EqGraph.push_makes_node {G : GlobalEnv} {Δ : KindEnv} {Γ : TyEnv} {eG eG' : EqGraph G Δ Γ}
   {T : Ty} {K : Kind} {j : G&Δ ⊢ T : K} :
   (eG.push ⟨T, K, j⟩) = eG' ->
-  T ∈ eG' := by sorry
+  T ∈ eG'
+  := by
+  unfold EqGraph.push;
+  split <;> (intro h; rw[<-h])
+  · assumption
+  · unfold instMembershipTyEqGraph; simp
+
+theorem EqGraph.push_keeps_edges {G : GlobalEnv} {Δ : KindEnv} {Γ : TyEnv} {eG eG' : EqGraph G Δ Γ}
+  {T : Ty} {K : Kind} {j : G&Δ ⊢ T : K} :
+  (eG.push ⟨T, K, j⟩) = eG' ->
+  eG.edges = eG'.edges
+  := by
+  unfold EqGraph.push;
+  split <;> (intro h; rw[<-h])
+
+-- Gets the representative node if the type exists
+def EqGraph.get_rep {G : GlobalEnv} {Δ : KindEnv} {Γ : TyEnv} (eG : EqGraph G Δ Γ) : Ty -> Option (Node G Δ)
+  := sorry
 
 
-def EqGraph.union {G : GlobalEnv} {Δ : KindEnv} {Γ : TyEnv} (eG : EqGraph G Δ Γ) (K : Kind) :
-  (T1 : Ty) -> (T2 : Ty) -> ((t : Term) ×' G&Δ, Γ ⊢ t : (T1 ~[K]~ T2)) -> EqGraph G Δ Γ := sorry
+def EqGraph.union {G : GlobalEnv} {Δ : KindEnv} {Γ : TyEnv} (eG : EqGraph G Δ Γ) (K : Kind)
+  (T1 : Ty) (T2 : Ty) (t : Term) (j : G&Δ, Γ ⊢ t : (T1 ~[K]~ T2)) : Option (EqGraph G Δ Γ) := do
+  let i1 <- eG.nodes.findIdx? (·.get_ty == T1)
+  let i2 <- eG.nodes.findIdx? (·.get_ty == T2)
+  match eG.nodes[i1]?, eG.nodes[i2]? with
+  | some n1, some n2 =>
+    sorry
+  | _, _ => none
+
 
 theorem EqGraph.union_adds_edge {G : GlobalEnv} {Δ : KindEnv} {Γ : TyEnv} {eG eG' : EqGraph G Δ Γ}  {K : Kind} {T1 T2 : Ty}
  (c : (t : Term) ×' G&Δ, Γ ⊢ t : (T1 ~[K]~ T2)) (h1 : T1 ∈ eG) (h2 : T2 ∈ eG) :
- eG.union K T1 T2 c = eG' ->
+ eG.union K T1 T2 c.1 c.2 = some eG' ->
  ∃ e ∈ eG'.edges, eG'.nodes[e.1]?.map (·.get_ty) = some T1 ∧ eG'.nodes[e.2.1]?.map (·.get_ty) = some T2 := by sorry
+
+theorem EqGraph.union_keeps_nodes {G : GlobalEnv} {Δ : KindEnv} {Γ : TyEnv} {eG eG' : EqGraph G Δ Γ}  {K : Kind} {T1 T2 : Ty}
+ (c : (t : Term) ×' G&Δ, Γ ⊢ t : (T1 ~[K]~ T2)) (h1 : T1 ∈ eG) (h2 : T2 ∈ eG) :
+ eG.union K T1 T2 c.1 c.2 = eG' ->
+ eG.nodes = eG'.nodes := by sorry
 
 
 def EqGraph.find {G : GlobalEnv} {Δ : KindEnv} {Γ : TyEnv} (eG : EqGraph G Δ Γ) : Ty -> Ty -> Option (Edge G Δ Γ) := sorry
 
-def EqGraph.get_parent {G : GlobalEnv} {Δ : KindEnv} {Γ : TyEnv} (eG : EqGraph G Δ Γ) : Ty -> Option (Node G Δ) := sorry
 
 def EqGraph.path {G : GlobalEnv} {Δ : KindEnv} {Γ : TyEnv} (eG : EqGraph G Δ Γ) : Ty -> Ty -> Option (List (Edge G Δ Γ)) := sorry
 
 def EqGraph.build_term {G : GlobalEnv} {Δ : KindEnv} {Γ : TyEnv} :
   List (Edge G Δ Γ) -> (t : Term) × (K : Kind) × (T1 : Ty) × (T2 : Ty) ×' (G&Δ, Γ ⊢ t : (T1 ~[K]~ T2)) := by sorry
 
-
-
--- ∀[K] ∀[K] ∀[K] (t#2 ~[K]~ t#1) -:> ((t#1 ~[K]~ t#0) -:> (t#2 ~[K]~ t#0))
 
 
 def Term.sym (K : Kind) : Term := Λ[K]Λ[K] λ[t#1 ~[K]~ t#0] (.cast (t#0 ~[K]~ t#2) #0 (refl! t#1))
@@ -130,6 +180,22 @@ def EqGraph.symm {G : GlobalEnv} {Δ : KindEnv} {Γ : TyEnv} {wf : ⊢ G} (t : T
        · simp
      · apply j⟩
 
+theorem seq_subst_rename_lemma {TA TB : Ty} :
+  TA⟨Ren.succ Ty⟩⟨Ren.succ Ty⟩[(su TB :: Subst.id Ty).lift] = TA⟨Ren.succ Ty⟩
+  := by
+    simp;
+    rw[Subst.compose_ren_left]; simp;
+    generalize σdef : (({ inner := fun n => re (n + 1) }) : LeanSubst.Subst Ty) = σ at *;
+    generalize rdef : Ren.succ Ty = r at *
+    have lem : r.to = σ := by
+      rw[<-rdef]; rw[<-σdef]
+      simp; unfold Subst.succ; simp
+    have lem2 := Subst.apply_stable lem (S := Ty) (T := Ty)
+    unfold SubstMap.smap; unfold instSubstMapTy;
+    unfold RenMap.rmap; unfold instRenMapTy; simp;
+    unfold SubstMap.smap at lem2; unfold instSubstMapTy at lem2;
+    unfold RenMap.rmap at lem2; unfold instRenMapTy at lem2; simp at lem2;
+    rw[lem2]
 
 def EqGraph.seq {G : GlobalEnv} {Δ : KindEnv} {Γ : TyEnv} {wf : ⊢ G}
   (t1 t2: Term) (K : Kind) (TA TB TC : Ty) (j1 : G&Δ, Γ ⊢ t1 : (TA ~[K]~ TB)) (j2 : G&Δ, Γ ⊢ t2 : (TB ~[K]~ TC)) :
@@ -147,25 +213,41 @@ def EqGraph.seq {G : GlobalEnv} {Δ : KindEnv} {Γ : TyEnv} {wf : ⊢ G}
            (P := ∀[K]((TA⟨Ren.succ Ty⟩⟨Ren.succ Ty⟩ ~[K]~ t#1) -:> (t#1 ~[K]~ t#0) -:> (TA⟨Ren.succ Ty⟩⟨Ren.succ Ty⟩ ~[K]~ t#0)))
         · apply Typing.appt (K := K) (P := ∀[K] ∀[K] (t#2 ~[K]~ t#1) -:> ((t#1 ~[K]~ t#0) -:> (t#2 ~[K]~ t#0)))
           · apply Typing.lamt
-            · sorry
+            · apply Kinding.all; apply Kinding.all; apply Kinding.all;
+              apply Kinding.arrow;
+              · apply Kinding.eq; apply Kinding.var; simp; apply Kinding.var; simp
+              · apply Kinding.arrow;
+                · apply Kinding.eq; apply Kinding.var; simp; apply Kinding.var; simp
+                · apply Kinding.eq; apply Kinding.var; simp; apply Kinding.var; simp
             · apply Typing.lamt
-              · sorry
+              · apply Kinding.all; apply Kinding.all; apply Kinding.arrow;
+                · apply Kinding.eq; apply Kinding.var; simp; apply Kinding.var; simp
+                · apply Kinding.arrow;
+                  · apply Kinding.eq; apply Kinding.var; simp; apply Kinding.var; simp
+                  · apply Kinding.eq; apply Kinding.var; simp; apply Kinding.var; simp
               · apply Typing.lamt
-                · apply Kinding.all; sorry
+                · apply Kinding.all; apply Kinding.arrow;
+                  · apply Kinding.eq; apply Kinding.var; simp; apply Kinding.var; simp
+                  · apply Kinding.arrow;
+                    · apply Kinding.eq; apply Kinding.var; simp; apply Kinding.var; simp
+                    · apply Kinding.eq; apply Kinding.var; simp; apply Kinding.var; simp
                 · apply Typing.lam
-                  · sorry
+                  · apply Kinding.eq; apply Kinding.var; simp; apply Kinding.var; simp
                   · apply Typing.lam
-                    · sorry
+                    · apply Kinding.eq; apply Kinding.var; simp; apply Kinding.var; simp
                     · apply Typing.cast (K := K) (A := t#1) (B := t#0)
-                      sorry
-                      apply Typing.var; simp; sorry
-                      apply Typing.var; simp; simp; sorry
-                      simp
+                      apply Kinding.eq; apply Kinding.var; simp; apply Kinding.var; simp
+                      apply Typing.var; simp;
+                      · apply Kinding.eq; apply Kinding.var; simp; apply Kinding.var; simp
+                      · apply Typing.var; simp; simp;
+                        apply Kinding.eq; apply Kinding.var; simp; apply Kinding.var; simp
+                      · simp
           · apply lemA
           · simp
 
         · apply lemB
-        · simp; rw[<-Ren.add_one]; sorry
+        · rw[Ty.subst_all, Ty.subst_arr, Ty.subst_eq, Ty.subst_var, seq_subst_rename_lemma];
+          rw[Ty.subst_arr, Ty.subst_eq, Ty.subst_eq]; rw[seq_subst_rename_lemma]; simp
 
       · apply lemC
       · simp
@@ -175,17 +257,17 @@ def EqGraph.seq {G : GlobalEnv} {Δ : KindEnv} {Γ : TyEnv} {wf : ⊢ G}
 
 
 def EqGraph.process_equation {G : GlobalEnv} {Δ : KindEnv} {Γ : TyEnv} (eG : EqGraph G Δ Γ) (K : Kind) :
-  (T1 : Ty) -> (G&Δ ⊢ T1 : K) -> (T2 : Ty) -> (G&Δ ⊢ T2 : K)  -> ((t : Term) ×' G&Δ, Γ ⊢ t : (T1 ~[K]~ T2)) -> EqGraph G Δ Γ
+  (T1 : Ty) -> (G&Δ ⊢ T1 : K) -> (T2 : Ty) -> (G&Δ ⊢ T2 : K)  -> ((t : Term) ×' G&Δ, Γ ⊢ t : (T1 ~[K]~ T2)) -> Option (EqGraph G Δ Γ)
 | T1, j1, T2, j2, ⟨c, j3⟩ =>
   let eG := eG.push ⟨T1, K, j1⟩
   let eG := eG.push ⟨T2, K, j2⟩
-  eG.union K T1 T2 ⟨c, j3⟩
+  eG.union K T1 T2 c j3
 
-def EqGraph.empty {G : GlobalEnv} {Δ : KindEnv} {Γ : TyEnv} : EqGraph G Δ Γ := { nodes := [], edges := []}
+def EqGraph.empty {G : GlobalEnv} {Δ : KindEnv} {Γ : TyEnv} : EqGraph G Δ Γ := { nodes := [], edges := [], parentD_lt := nofun, rankD_lt := nofun}
 
 def EqGraph.build_coercion {G : GlobalEnv} {Δ : KindEnv} {Γ : TyEnv} (eG : EqGraph G Δ Γ) (T1 T2 : Ty) : Option (Edge G Δ Γ) :=  do
-  let p1 <- eG.get_parent T1
-  let p2 <- eG.get_parent T2
+  let p1 <- eG.get_rep T1
+  let p2 <- eG.get_rep T2
   if p1.get_ty == p2.get_ty
   then do
     let T1_to_p1 <- eG.path T1 p1.get_ty
